\documentclass{article}
\usepackage{amsmath}
\usepackage{amssymb}
\usepackage{ragged2e}
\usepackage[utf8]{inputenc}
\DeclareMathOperator{\Q}{\mathbb{Q}}
\DeclareMathOperator{\R}{\mathbb{R}}
\DeclareMathOperator{\E}{\mathbb{E}}
\DeclareMathOperator{\Prop}{\mathbb{P}}
\DeclareMathOperator{\softmax}{softmax}
\DeclareMathOperator{\1}{1\!\!1}
\DeclareMathOperator{\Bias}{Bias}
\DeclareMathOperator{\MSE}{MSE}
\DeclareMathOperator{\qed}{QED}
\begin{document}
\section{}
z.z. \(s \mapsto S_i(v)\) ist probability mass function.\\
bew.
\begin{flalign*}
\sum_{i=1}^n S_i(v) = \sum_{i=1}^n {e^{v_i}\over \sum_{j=1}^n e^{v_j}} =  { \sum_{i=1}^n e^{v_i}\over \sum_{i=1}^n e^{v_i}} = 1\\\qed
\end{flalign*}
z.z. \(S_j(w)=S_j(v)\) f√ºr \(w_i = v_i +c\)\\
bew.
\begin{flalign*}
S_j(w)= {e^{w_j}\over \sum_{i=1}^n e^{w_i}} = {e^{x_j+c}\over \sum_{i=1}^n e^{v_i+c}}= {e^c e^{x_j}\over \sum_{i=1}^n e^c e^{v_i}}= {e^c e^{x_j}\over e^c \sum_{i=1}^n e^{v_i}}= { e^{x_j}\over\sum_{i=1}^n  e^{v_i}}=S_j(v)\\\qed
\end{flalign*}
z.z. \({\partial S_j(v) \over \partial v_i }=S_j(v)(\delta_{ij}-S_i(v))\)\\
bew.
\begin{flalign*}
{\partial S_j(v) \over \partial v_i }&={\partial \over \partial v_i }{e^{v_j}\over \sum_{k=1}^n e^{v_k}} \\
&={\left({\partial \over \partial v_i} e^{v_j}\right)\sum_{k=1}^n e^{v_k}-e^{v_j}\left({\partial \over \partial v_i }\sum_{k=1}^n e^{v_k}\right)\over\left(\sum_{k=1}^n e^{v_k}\right)^2} \\
&={\delta _{ij}e^{v_j}\sum_{k=1}^n e^{v_k}-e^{v_j}e^{v_i})\over\left(\sum_{k=1}^n e^{v_k}\right)^2}\\
&=\delta_{ij} S_j(v)-S_i(v) S_j(v) \\
&= S_j(v)(\delta_{ij}-S_i(v))\\\qed
\end{flalign*}\newpage
\section{}
Berechne \({\partial H(t,q)\over\partial q_j}={\partial\over\partial q_j}\left(-\sum_{i=1}^n t_i log(q_i)\right)=-{t_j\over q_j}\)\\
z.z. \({\partial H(t,\softmax(v))\over\partial v_i}=S_i(v)-t_i\)\\
bew.
\begin{flalign*}
{\partial H(t,\softmax(v))\over\partial v_i}&={\partial H(t,\softmax(v))\over\partial \softmax(v)}{\partial \softmax(v)\over\partial v_i}\\
&={\left(-{t_j\over S_j(v)}\right)_{j=1}^n}^\top\left(S_j(v)(\delta_{ij}-S_i(v))\right)_{j=1}^n\\
&=\sum_{j=1}^n -{t_j\over S_j(v)}S_j(v)(\delta_{ij}-S_i(v))\\
&=\sum_{j=1}^n (t_j S_i(v)-t_j\delta_{ij})\\
&=\sum_{j=1}^n t_j S_i(v)-t_i\\
&=\left(\sum_{j=1}^n t_j\right) S_i(v)-t_i\\
&=S_i(v)-t_i\\\qed
\end{flalign*}
\end{document}